Some work on the theorem

doc/formalization/Catala.Translation.fst
@@ -49,27 +49,22 @@ let typ_process_exceptions_f (tau: L.ty)
 
 (**** Main translation *)
 
-let build_default_translation_aux
-  (e: D.exp)
-  (exceptions: list D.exp{exceptions << e})
-  (just: D.exp{just << e})
-  (cons: D.exp{cons << e})
-  (tau: D.ty)
-  (translate_exp: (e':D.exp{e' << e}) -> L.exp)
-  (translate_exp_list: (l:list D.exp{l << e}) -> list L.exp)
+let build_default_translation
+  (exceptions: list L.exp)
+  (just: L.exp)
+  (cons: L.exp)
+  (tau: L.ty)
   =
-  let tau' = translate_ty tau in
   L.EMatchOption
     (L.EFoldLeft
-      (process_exceptions_f tau')
-      L.ENone (L.TOption tau')
-      (L.EList (translate_exp_list exceptions)) (L.TArrow L.TUnit tau'))
-    tau'
+      (process_exceptions_f tau)
+      L.ENone (L.TOption tau)
+      (L.EList exceptions) (L.TArrow L.TUnit tau))
+    tau
     (L.EIf
-      (translate_exp just)
-      (translate_exp cons)
+      just cons
       (L.ELit (L.LError L.EmptyError)))
-    (L.EAbs (L.Named 0) tau' (L.EVar 0))
+    (L.EAbs (L.Named 0) tau (L.EVar 0))
 
 let rec translate_exp (e: D.exp) : Tot L.exp = match e with
   | D.EVar x -> L.EVar x
@@ -82,30 +77,15 @@ let rec translate_exp (e: D.exp) : Tot L.exp = match e with
     (translate_exp e2)
     (translate_exp e3)
   | D.EDefault exceptions just cons tau ->
-    build_default_translation_aux e exceptions just cons tau translate_exp translate_exp_list
+    build_default_translation
+      (translate_exp_list exceptions)
+      (translate_exp just)
+      (translate_exp cons)
+      (translate_ty tau)
 and translate_exp_list (l: list D.exp) : Tot (list L.exp) =
   match l with
   | [] -> []
   | hd::tl -> (L.EAbs L.Silent L.TUnit (translate_exp hd))::(translate_exp_list tl)
-
-let build_default_translation
-  (exceptions: list D.exp)
-  (just: D.exp)
-  (cons: D.exp)
-  (tau: D.ty)
-  =
-  let e = D.EDefault exceptions just cons tau in
-  assume(exceptions << e);
-  assume(just << e);
-  assume(cons << e);
-  build_default_translation_aux
-    e
-    exceptions
-    just
-    cons
-    tau
-    translate_exp
-    translate_exp_list
 
 let translate_env (g: D.env) : Tot L.env =
  FunctionalExtensionality.on_dom L.var_name
@@ -231,54 +211,31 @@ let is_stepping_agnostic_lift (f:(L.exp -> not_l_value)) = forall (e: L.exp).
 
 let stepping_agnostic_lift = f:(L.exp -> not_l_value){is_stepping_agnostic_lift f}
 
-#push-options "--fuel 15 --ifuel 2 --z3rlimit 30"
-let exceptions_lift
-  (hd: D.exp)
-  (just: D.exp)
-  (cons: D.exp)
-  (tau: D.ty)
+#push-options "--fuel 4 --ifuel 1"
+let default_translation_head_lift
+  (ltl: list L.exp)
+  (ljust: L.exp)
+  (lcons: L.exp)
+  (ltau: L.ty)
     : Tot stepping_agnostic_lift
   =
-  let tau' = translate_ty tau in
-  let aux (tl: L.exp) : not_l_value =
-      L.EMatchOption
-       (L.EFoldLeft
-         (process_exceptions_f tau')
-         L.ENone (L.TOption tau')
-         (L.EList (match tl with
-          | L.EList l -> (translate_exp hd)::l
-          | _ -> [translate_exp hd;tl]
-         )) (L.TArrow L.TUnit tau'))
-      tau'
-        (L.EIf
-          (translate_exp just)
-          (translate_exp cons)
-        (L.ELit (L.LError L.EmptyError)))
-      (L.EAbs (L.Named 0) tau' (L.EVar 0))
-   in
-   let aux_lemma (e: L.exp) : Lemma (step_lift_commute_non_value aux e) =
-     if L.is_value e then () else
-     match e, L.step e with
-     | L.EList l, _ -> admit()
-     | _, None -> admit()
-     | _, Some e' -> admit()
-   in
-   Classical.forall_intro aux_lemma;
-   assert(is_stepping_agnostic_lift aux);
-   aux
-
-#push-options "--fuel 15 --ifuel 8 --z3rlimit 150"
-let exceptions_lift_lemma
-  (hd: D.exp)
-  (just: D.exp)
-  (cons: D.exp)
-  (tau: D.ty)
-  (tl: list D.exp)
-    : Lemma (
-      exceptions_lift hd just cons tau (build_default_translation tl just cons tau) ==
-      build_default_translation (hd::tl) just cons tau)
-  =
-  admit()
+  let f : L.exp -> not_l_value = fun lhd ->
+    build_default_translation ((L.EAbs L.Silent L.TUnit lhd)::ltl) ljust lcons ltau
+  in
+  let aux (e: L.exp) : Lemma(step_lift_commute_non_value f e) =
+    if L.is_value e then () else
+    match L.step e with
+    | None ->
+      let open FStar.Tactics in
+      // TODO: this is false with one step but true with multiple steps!
+      assume(L.step (f e) = None)
+    | Some e' ->
+      let open FStar.Tactics in
+      assume(L.step (f e) = Some (f e'))
+  in
+  Classical.forall_intro aux;
+  assert(is_stepping_agnostic_lift f);
+  f
 #pop-options
 
 let rec l_values_dont_step (e: L.exp) : Lemma
@@ -374,7 +331,7 @@ let translation_correctness_value (e: D.exp) : Lemma
     ((D.is_value e) <==> (L.is_value (translate_exp e)))
   = ()
 
-#push-options "--fuel 2 --ifuel 1 --z3rlimit 50"
+#push-options "--fuel 2 --ifuel 1 --z3rlimit 1000"
 let rec translation_correctness_step (e: D.exp) : Pure nat
     (requires (Some? (D.step e)))
     (ensures (fun n -> multiple_l_steps (translate_exp e) (translate_exp (Some?.v (D.step e))) n))
@@ -463,7 +420,11 @@ and translation_correctness_exceptions_left_to_right_step
       ))
       (ensures (fun n ->
         multiple_l_steps
-          (build_default_translation exceptions just cons tau)
+          (build_default_translation
+            (translate_exp_list exceptions)
+            (translate_exp just)
+            (translate_exp cons)
+            (translate_ty tau))
           (translate_exp
             (Some?.v (D.step_exceptions_left_to_right e exceptions just cons tau))) n
       ))
@@ -472,28 +433,44 @@ and translation_correctness_exceptions_left_to_right_step
   match exceptions with
   | [] -> 0
   | hd::tl ->
+    let ljust = translate_exp just in
+    let lcons = translate_exp cons in
+    let ltl = translate_exp_list tl in
+    let ltau = translate_ty tau in
+    let lhd = translate_exp hd in
     if D.is_value hd then begin
       match D.step_exceptions_left_to_right e tl just cons tau with
       | Some (D.ELit D.LConflictError) -> admit()
       | Some (D.EDefault tl' just' cons' tau') ->
         assume(just = just' /\ cons = cons' /\ tau = tau');
+        let ltl' = translate_exp_list tl' in
         let n_tl = translation_correctness_exceptions_left_to_right_step e tl just cons tau in
         assert(multiple_l_steps
-          (build_default_translation tl just cons tau)
-          (build_default_translation tl' just cons tau) n_tl);
-        lift_multiple_l_steps
-          (build_default_translation tl just cons tau)
-          (build_default_translation tl' just cons tau)
-          n_tl (exceptions_lift hd cons just tau);
-        exceptions_lift_lemma hd just cons tau tl;
-        exceptions_lift_lemma hd just cons tau tl';
-        assert(multiple_l_steps
-          (build_default_translation (hd::tl) just cons tau)
-          (build_default_translation (hd::tl') just cons tau) n_tl);
+          (build_default_translation ltl ljust lcons ltau)
+          (build_default_translation ltl' ljust lcons ltau) n_tl);
+        assume(multiple_l_steps
+          (build_default_translation (lhd::ltl) ljust  lcons ltau)
+          (build_default_translation (lhd::ltl') ljust lcons ltau) n_tl);
+        assume((translate_exp
+            (Some?.v (D.step_exceptions_left_to_right e exceptions just cons tau)))
+            ==
+             (build_default_translation
+            (lhd::ltl')
+            (translate_exp just)
+            (translate_exp cons)
+            (translate_ty tau)));
         n_tl
-      | None -> 0
     end else begin
-      admit()
+      match D.step hd with
+      | Some (D.ELit D.LConflictError) -> admit()
+      | Some stepped_hd ->
+         let stepped_hd' = translate_exp stepped_hd in
+         let n_hd = translation_correctness_step hd in
+         let hd' = translate_exp hd in
+         let tl' = translate_exp_list tl in
+         lift_multiple_l_steps hd' stepped_hd' n_hd
+           (default_translation_head_lift tl' ljust lcons ltau);
+         n_hd
     end
 
 (*** Wrap-up theorem  *)
